[WIP] type check

theories/Extraction/TypeCheck.v
@@ -1,8 +1,53 @@
+From Coq Require Import Morphisms_Relations.
 From Mcltt Require Import Base LibTactics.
-From Mcltt.Core Require Import Completeness NbE Soundness SystemOpt.
+From Mcltt.Core Require Import
+  Completeness
+  Completeness.Consequences.Inversions
+  Completeness.Consequences.Types
+  Completeness.FundamentalTheorem
+  Completeness.LogicalRelation
+  NbE
+  Semantic.Consequences
+  Semantic.Realizability
+  Soundness
+  SystemOpt.
 From Mcltt.Extraction Require Import NbE.
 From Equations Require Import Equations.
 Import Domain_Notations.
+
+Definition sumbool_failable_bind {A B} (ab : {A} + {B}) {C D : Prop} (fail : B -> D) (next : A -> {C} + {D}) :=
+  match ab with
+  | left a => next a
+  | right b => right (fail b)
+  end.
+
+Notation "'let*b' a ':=' ab 'while' fail 'in' next" := (sumbool_failable_bind ab fail (fun a => next)) (at level 0, a pattern, next at level 10, right associativity, only parsing).
+Notation "'pureb' a" := (left a) (at level 0, only parsing).
+
+Definition sumor_failable_bind {A B} (ab : A + {B}) {C} {D : Prop} (fail : B -> D) (next : A -> C + {D}) :=
+  match ab with
+  | inleft a => next a
+  | inright b => inright (fail b)
+  end.
+
+Notation "'let*o' a ':=' ab 'while' fail 'in' next" := (sumor_failable_bind ab fail (fun a => next)) (at level 0, a pattern, next at level 10, right associativity, only parsing).
+Notation "'pureo' a" := (inleft a) (at level 0, only parsing).
+
+Definition sumbool_sumor_failable_bind {A B} (ab : {A} + {B}) {C} {D : Prop} (fail : B -> D) (next : A -> C + {D}) :=
+  match ab with
+  | left a => next a
+  | right b => inright (fail b)
+  end.
+
+Notation "'let*b->o' a ':=' ab 'while' fail 'in' next" := (sumbool_sumor_failable_bind ab fail (fun a => next)) (at level 0, a pattern, next at level 10, right associativity, only parsing).
+
+Definition sumor_sumbool_failable_bind {A B} (ab : A + {B}) {C} {D : Prop} (fail : B -> D) (next : A -> {C} + {D}) :=
+  match ab with
+  | inleft a => next a
+  | inright b => right (fail b)
+  end.
+
+Notation "'let*o->b' a ':=' ab 'while' fail 'in' next" := (sumor_sumbool_failable_bind ab fail (fun a => next)) (at level 0, a pattern, next at level 10, right associativity, only parsing).
 
 (* Section nf_subsumption_dec. *)
 (*   #[local] *)
@@ -20,49 +65,41 @@ Import Domain_Notations.
 (*   #[tactic=impl_obl_tac] *)
 (*   Equations nf_subsumption_dec A A' : {nf_subsumption A A'} + {~ nf_subsumption A A'} := *)
 (*   | n{{{ Type@i }}}, n{{{ Type@j }}} => *)
-(*       match Compare_dec.le_lt_dec i j with *)
-(*       | left _ => left _ *)
-(*       | right _ => right _ *)
-(*       end *)
+(*       let*b _ := Compare_dec.le_lt_dec i j while _ in *)
+(*       pureb _ *)
 (*   (* Here we have a separate clause for n{{{ Type@i }}} so that we can extract a more efficient code *) *)
 (*   | n{{{ Type@i }}}, _ => right _ *)
 (*   | A, A' => *)
-(*       match nf_eq_dec A A' with *)
-(*       | left _ => left _ *)
-(*       | right _ => right _ *)
-(*       end. *)
+(*       let*b _ := nf_eq_dec A A' while _ in *)
+(*       pureb _. *)
 (* End nf_subsumption_dec. *)
 
 (* Section conversion_dec. *)
 (*   #[local] *)
 (*   Ltac impl_obl_tac := *)
 (*     match goal with *)
-(*     | |- nbe_order ?G ?M ?A => *)
+(*     | |- nbe_order _ _ _ => *)
 (*         (on_all_hyp: fun H => apply soundness in H); *)
 (*         destruct_conjs; *)
 (*         eapply nbe_order_sound; eassumption *)
-(*     | |- False => *)
-(*         (on_all_hyp: fun H => apply completeness in H); *)
+(*     | |- _ <> _ -> ~ {{ ~_ ⊢ ~_ ≈ ~_ : ~_ }} => *)
+(*         intros ? ?%completeness; *)
 (*         destruct_conjs; *)
 (*         functional_nbe_rewrite_clear; *)
 (*         congruence *)
-(*     | _ => *)
+(*     | |- {{ ~_ ⊢ ~_ ≈ ~_ : ~_ }} => *)
 (*         (on_all_hyp: fun H => apply soundness in H); *)
 (*         destruct_conjs; *)
 (*         functional_nbe_rewrite_clear; *)
-(*         mauto *)
+(*         mautosolve *)
 (*     end. *)
-
 (*   #[tactic="impl_obl_tac"] *)
 (*   Equations conversion_dec G A M (HM : {{ G ⊢ M : A }}) M' (HM' : {{ G ⊢ M' : A }}) : { {{ G ⊢ M ≈ M' : A }} } + { ~ {{ G ⊢ M ≈ M' : A }} } := *)
 (*   | G, A, M, HM, M', HM' => *)
 (*       let (W, HW) := nbe_impl G M A _ in *)
 (*       let (W', HW') := nbe_impl G M' A _ in *)
-(*       match nf_eq_dec W W' with *)
-(*       | left _ => left _ *)
-(*       | right _ => right _ *)
-(*       end. *)
-(*   Next Obligation. impl_obl_tac. Qed. *)
+(*       let*b _ := nf_eq_dec W W' while _ in *)
+(*       pureb _. *)
 (* End conversion_dec. *)
 
 (* Section typ_subsumption_dec. *)
@@ -83,8 +120,10 @@ Import Domain_Notations.
 (*         assert {{ G ⊢ W' : Type@i }} by (gen_presups; eassumption); *)
 (*         assert {{ G ⊢ W ⊆ W' }} by mauto; *)
 (*         etransitivity; *)
-(*         mauto *)
-(*     | H: ~ (nf_subsumption ?W ?W') |- ~ {{ ~?G ⊢ ~?A ⊆ ~?A' }} => *)
+(*         mautosolve *)
+(*     | |- ~ (nf_subsumption ?W ?W') -> ~ {{ ~?G ⊢ ~?A ⊆ ~?A' }} => *)
+(*         let H := fresh "H" in *)
+(*         intro H; *)
 (*         contradict H; *)
 (*         apply completeness_for_typ_subsumption in H; *)
 (*         destruct_conjs; *)
@@ -97,8 +136,459 @@ Import Domain_Notations.
 (*   | G, i, A, HA, A', HA' => *)
 (*       let (W, HW) := nbe_impl G A {{{ Type@i }}} _ in *)
 (*       let (W', HW') := nbe_impl G A' {{{ Type@i }}} _ in *)
-(*       match nf_subsumption_dec W W' with *)
-(*       | left _ => left _ *)
-(*       | right _ => right _ *)
-(*       end. *)
+(*       let*b _ := nf_subsumption_dec W W' while _ in *)
+(*       pureb _. *)
 (* End typ_subsumption_dec. *)
+
+Section lookup.
+  #[local]
+  Ltac impl_obl_tac1 :=
+    match goal with
+    | |- ~_ => intro
+    | H: {{ ⊢ ~_, ~_ }} |- _ => inversion_clear H
+    | H: {{ # _ : ~_ ∈ ⋅ }} |- _ => inversion_clear H
+    | H: {{ # (S _) : ~_ ∈ ~_, ~_ }} |- _ => inversion_clear H
+    end.
+
+  #[local]
+  Ltac impl_obl_tac :=
+    intros;
+    repeat impl_obl_tac1;
+    intuition (mauto 4).
+
+  #[tactic="impl_obl_tac"]
+  Equations lookup G (HG : {{ ⊢ G }}) x : { A | {{ #x : A ∈ G }} } + { forall A, ~ {{ #x : A ∈ G }} } :=
+  | {{{ G, A }}}, HG, x with x => {
+    | 0 => pureo (exist _ {{{ A[Wk] }}} _)
+    | S x' =>
+        let*o (exist _ B _) := lookup G _ x' while _ in
+        pureo (exist _ {{{ B[Wk] }}} _)
+    }
+  | {{{ ⋅ }}}, HG, x => inright _.
+End lookup.
+
+Axiom TODO : False.
+
+Tactic Notation "TODOtac" string(_unused) := exfalso; exact TODO.
+
+Section pi_conversion.
+  #[local]
+  Ltac impl_obl_tac :=
+    simpl in *;
+    match goal with
+    | |- nbe_order ?G ?M ?A =>
+        (on_all_hyp: fun H => apply soundness in H);
+        destruct_conjs;
+        eapply nbe_order_sound; eassumption
+    | H: nbe ?G ?C {{{ Type@?i }}} ?W |- forall j A B, ~ {{ ~?G ⊢ Π A B ≈ ~?C : Type@j }} =>
+        intros * ?;
+        (on_all_hyp: fun H => apply soundness in H);
+        destruct_conjs;
+        functional_nbe_rewrite_clear;
+        assert {{ G ⊢ Π A B ≈ W : Type@(max i j) }} by mauto;
+        assert {{ G ⊨ Π A B ≈ W : Type@(max i j) }} as [env_relG] by mauto using completeness_fundamental_exp_eq;
+        destruct_conjs;
+        assert (exists p p', initial_env G p /\ initial_env G p' /\ {{ Dom p ≈ p' ∈ env_relG }}) as [p [? [? []]]] by eauto using per_ctx_then_per_env_initial_env;
+        functional_initial_env_rewrite_clear;
+        (on_all_hyp: destruct_rel_by_assumption env_relG);
+        destruct_by_head rel_typ;
+        invert_rel_typ_body;
+        destruct_by_head rel_exp;
+        invert_rel_typ_body;
+        destruct_conjs;
+        match_by_head1 per_univ_elem invert_per_univ_elem
+    | _ => idtac "upwg"; show_hyps; show_goal
+    end.
+
+  #[tactic="impl_obl_tac"]
+  Equations pi_conversion G i C (HC : {{ G ⊢ C : Type@i }}) : { '(A, B) | {{ G ⊢ Π A B ≈ C : Type@i }} } + { forall j A B, ~{{ G ⊢ Π A B ≈ C : Type@j }} } :=
+  | G, i, C, HC with nbe_impl G C {{{ Type@i }}} _ => {
+    | (exist _ n{{{ Π W1 W2 }}} _) => pureo (exist _ (nf_to_exp W1, nf_to_exp W2) _)
+    | _ => inright _
+    }
+  .
+
+  Next Obligation.
+    (on_all_hyp: fun H => apply soundness in H).
+    destruct_conjs.
+    functional_nbe_rewrite_clear.
+    mauto.
+  Qed.
+
+  Next Obligation.
+    TODOtac "Pi is never equivalent to a neutral term".
+  Qed.
+End pi_conversion.
+
+Section type_check.
+  Inductive type_check_order : exp -> Prop :=
+  | tc_typ : forall {i}, min_level_infer_order {{{ Type@i }}} -> type_check_order {{{ Type@i }}}
+  | tc_nat : min_level_infer_order {{{ ℕ }}} -> type_check_order {{{ ℕ }}}
+  | tc_zero : type_check_order {{{ zero }}}
+  | tc_succ : forall {M}, type_check_order M -> type_check_order {{{ succ M }}}
+  | tc_natrec : forall {A MZ MS M}, min_type_infer_order {{{ rec M return A | zero -> MZ | succ -> MS end }}} -> type_check_order {{{ rec M return A | zero -> MZ | succ -> MS end }}}
+  | tc_pi : forall {A B}, min_level_infer_order {{{ Π A B }}} -> type_check_order {{{ Π A B }}}
+  | tc_fn : forall {A M}, min_level_infer_order A -> type_check_order M -> type_check_order {{{ λ A M }}}
+  | tc_app : forall {M N}, min_type_infer_order {{{ M N }}} -> type_check_order {{{ M N }}}
+  | tc_vlookup : forall {x}, min_type_infer_order {{{ #x }}} -> type_check_order {{{ #x }}}
+  with min_type_infer_order : exp -> Prop :=
+  | mti_typ : forall {i}, min_level_infer_order {{{ Type@i }}} -> min_type_infer_order {{{ Type@i }}}
+  | mti_nat : min_level_infer_order {{{ ℕ }}} -> min_type_infer_order {{{ ℕ }}}
+  | mti_zero : min_type_infer_order {{{ zero }}}
+  | mti_succ : forall {M}, type_check_order M -> min_type_infer_order {{{ succ M }}}
+  | mti_natrec : forall {A MZ MS M}, type_check_order M -> min_level_infer_order A -> type_check_order MZ -> type_check_order MS -> min_type_infer_order {{{ rec M return A | zero -> MZ | succ -> MS end }}}
+  | mti_pi : forall {A B}, min_level_infer_order {{{ Π A B }}} -> min_type_infer_order {{{ Π A B }}}
+  | mti_fn : forall {A M}, min_level_infer_order A -> min_type_infer_order M -> min_type_infer_order {{{ λ A M }}}
+  | mti_app : forall {M N}, min_type_infer_order M -> type_check_order N -> min_type_infer_order {{{ M N }}}
+  | mti_vlookup : forall {x}, min_type_infer_order {{{ #x }}}
+  with min_level_infer_order : exp -> Prop :=
+  | mlv_typ : forall {i}, min_level_infer_order {{{ Type@i }}}
+  | mlv_nat : min_level_infer_order {{{ ℕ }}}
+  | mlv_zero : min_level_infer_order {{{ zero }}}
+  | mlv_succ : forall {M}, min_level_infer_order {{{ succ M }}}
+  | mlv_natrec : forall {A MZ MS M}, min_type_infer_order {{{ rec M return A | zero -> MZ | succ -> MS end }}} -> min_level_infer_order {{{ rec M return A | zero -> MZ | succ -> MS end }}}
+  | mlv_pi : forall {A B}, min_level_infer_order A -> min_level_infer_order B -> min_level_infer_order {{{ Π A B }}}
+  | mlv_fn : forall {A M}, min_level_infer_order {{{ λ A M }}}
+  | mlv_app : forall {M N}, min_level_infer_order M -> min_level_infer_order N -> min_level_infer_order {{{ M N }}}
+  | mlv_vlookup : forall {x}, min_type_infer_order {{{ #x }}} -> min_level_infer_order {{{ #x }}}
+  .
+
+  #[local]
+  Ltac impl_obl_tac :=
+    destruct_conjs;
+    match goal with
+    | |- {{ ⊢ ~_ }} => gen_presups; mautosolve 4
+    | H: {{ ~?G ⊢ ~?A : Type@?i }} |- {{ ~?G ⊢ ~?A : Type@(Nat.max ?i ?j) }} => apply lift_exp_max_left; mautosolve 4
+    | H: {{ ~?G ⊢ ~?A : Type@?j }} |- {{ ~?G ⊢ ~?A : Type@(Nat.max ?i ?j) }} => apply lift_exp_max_right; mautosolve 4
+    | |- {{ ~_ ⊢ ~_ : ~_ }} => gen_presups; mautosolve 4
+    | |- type_check_order _ => progressive_inversion; eassumption
+    | |- min_type_infer_order _ => progressive_inversion; eassumption
+    | |- min_level_infer_order _ => progressive_inversion; eassumption
+    | _ => show_hyps; show_goal
+    end.
+
+  Definition inspect {A} (a : A) : {b | a = b} := exist _ a eq_refl.
+
+  #[tactic="impl_obl_tac"]
+  Equations type_check G i A (HA : {{ G ⊢ A : Type@i }}) M (H : type_check_order M) : { {{ G ⊢ M : A }} } + { ~ {{ G ⊢ M : A }} } by struct H :=
+  | G, i, A, HA, M, H with M => {
+    | {{{ Type@j }}} =>
+        let*o->b (exist _ k _) := min_level_infer G {{{ Type@j }}} _ while _ in
+        let*b _ := typ_subsumption_dec G (max i (S k)) {{{ Type@k }}} _ A _ while _ in
+        pureb _
+    | {{{ ℕ }}} =>
+        let*o->b (exist _ j _) := min_level_infer G {{{ ℕ }}} _ while _ in
+        let*b _ := typ_subsumption_dec G (max i (S j)) {{{ Type@j }}} _ A _ while _ in
+        pureb _
+    | {{{ zero }}} =>
+        let*b _ := typ_subsumption_dec G i {{{ ℕ }}} _ A HA while _ in
+        pureb _
+    | {{{ succ M' }}} =>
+        let*b _ := typ_subsumption_dec G i {{{ ℕ }}} _ A HA while _ in
+        let*b _ := type_check G 0 {{{ ℕ }}} _ M' _ while _ in
+        pureb _
+    | {{{ rec M' return A' | zero -> MZ | succ -> MS end }}} =>
+        let*o->b (exist _ A''j _) := min_type_infer G _ {{{ rec M' return A' | zero -> MZ | succ -> MS end }}} _ while _ in
+        let*b _ := typ_subsumption_dec G (max i (snd A''j)) (fst A''j) _ A _ while _ in
+        pureb _
+    | {{{ Π B' C' }}} =>
+        let*o->b (exist _ j _) := min_level_infer G {{{ Π B' C' }}} _ while _ in
+        let*b _ := typ_subsumption_dec G (max i (S j)) {{{ Type@j }}} _ A _ while _ in
+        pureb _
+    | {{{ λ B' M' }}} with pi_conversion G i A HA => {
+      | inleft (exist _ BC _) with inspect BC => {
+        | exist _ (B, C) _ =>
+            let*o->b (exist _ j _) := min_level_infer G {{{ B' }}} _ while _ in
+            let*b _ := conversion_dec G {{{ Type@(max i j) }}} B' _ B _ while _ in
+            let*b _ := type_check {{{ G, B' }}} i C _ M' _ while _ in
+            pureb _
+        }
+      | inright _ => right _
+      }
+    | {{{ M' N' }}} with min_type_infer G _ M' _ => {
+      | inleft (exist _ C'j _) with inspect C'j => {
+        | exist _ (C', j) _ with pi_conversion G j C' _ => {
+          | inleft (exist _ B'A' _) with inspect B'A' => {
+            | exist _ (B', A') _ =>
+                let*b _ := type_check G j B' _ N' _ while _ in
+                let*b _ := typ_subsumption_dec G (max i j) A' _ A _ while _ in
+                pureb _
+            }
+          | inright _ => right _
+          }
+        }
+      | inright HnotM' => _
+      }
+    | {{{ #x }}} =>
+        let*o->b (exist _ A'j _) := min_type_infer G _ {{{ #x }}} _ while _ in
+        let*b _ := typ_subsumption_dec G (max i (snd A'j)) (fst A'j) _ A _ while _ in
+        pureb _
+    | _ =>
+        match (_ : False) with
+        end
+    }
+  with min_type_infer G (HG : {{ ⊢ G }}) M (H : min_type_infer_order M) : { '(pair A i) | {{ G ⊢ M : A }} /\ {{ G ⊢ A : Type@i }} /\ (forall A', {{ G ⊢ M : A' }} -> {{ G ⊢ A ⊆ A' }}) } + { forall A, ~ {{ G ⊢ M : A }} } by struct H :=
+  | G, HG, M, H with M => {
+    | {{{ Type@j }}} =>
+        let*o (exist _ i _) := min_level_infer G {{{ Type@j }}} _ while _ in
+        pureo (exist _ ({{{ Type@i }}}, S i) _)
+    | {{{ ℕ }}} => 
+        let*o (exist _ i _) := min_level_infer G {{{ ℕ }}} _ while _ in
+        pureo (exist _ ({{{ Type@i }}}, S i) _)
+    | {{{ rec M' return A' | zero -> MZ | succ -> MS end }}} =>
+        let*b->o _ := type_check G 0 {{{ ℕ }}} _ M' _ while _ in
+        let*o (exist _ j _) := min_level_infer {{{ G, ℕ }}} A' _ while _ in
+        let*b->o _ := type_check G j {{{ A'[Id,,zero] }}} _ MZ _ while _ in
+        let*b->o _ := type_check {{{ G, ℕ, A' }}} j {{{ A'[Wk∘Wk,,succ #1] }}} _ MS _ while _ in
+        pureo (exist _ ({{{ A'[Id,,M'] }}}, S j) _)
+    | {{{ Π B C }}} =>
+        let*o (exist _ i _) := min_level_infer G B _ while _ in
+        let*o (exist _ j _) := min_level_infer {{{ G, B }}} C _ while _ in
+        let k := max i j in
+        pureo (exist _ ({{{ Type@k }}}, S k) _)
+    | {{{ λ A' M' }}} =>
+        let*o (exist _ j _) := min_level_infer G A' _ while _ in
+        let*o (exist _ B'k _) := min_type_infer {{{ G, A' }}} _ M' _ while _ in
+        pureo (exist _ ({{{ Π A' ~(fst B'k) }}}, max j (snd B'k)) _)
+    | {{{ #x }}} =>
+        let*o (exist _ A _) := lookup G _ x while _ in
+        let*o (exist _ i _) := min_level_infer G A _ while _ in
+        pureo (exist _ (A, i) _)
+    | _ =>
+        match (_ : False) with
+        end
+    }
+  with min_level_infer G A (H : min_level_infer_order A) : { i | {{ G ⊢ A : Type@i }} /\ (forall j, {{ G ⊢ A : Type@j }} -> i <= j) } + { forall i, ~ {{ G ⊢ A : Type@i }} } by struct H :=
+  | G, A, H with A => {
+    | {{{ Type@j }}} => pureo (exist _ (S j) _)
+    | {{{ ℕ }}} => pureo (exist _ 0 _)
+    | {{{ Π B C }}} =>
+        let*o (exist _ i _) := min_level_infer G B _ while _ in
+        let*o (exist _ j _) := min_level_infer {{{ G, B }}} C _ while _ in
+        pureo (exist _ (max i j) _)
+    | _ =>
+        match (_ : False) with
+        end
+    }
+  .
+
+  Next Obligation with mautosolve.
+    enough {{ G ⊢ ℕ ⊆ A }} by contradiction.
+    eauto using wf_zero_inversion.
+  Qed.
+
+  Next Obligation with mautosolve.
+    enough {{ G ⊢ ℕ ⊆ A }} by contradiction.
+    eapply wf_succ_inversion; eauto.
+  Qed.
+
+  Next Obligation with mautosolve.
+    enough {{ G ⊢ M' : ℕ }} by contradiction.
+    eapply wf_succ_inversion'...
+  Qed.
+
+  Next Obligation with mautosolve.
+    intuition.
+  Qed.
+
+  Lemma vlookup_uniqueness : forall {Γ x A A'},
+      {{ #x : A ∈ Γ }} ->
+      {{ #x : A' ∈ Γ }} ->
+      A = A'.
+  Proof.
+    intros * HA.
+    dependent induction HA generalizing A'; inversion_clear 1; eauto.
+    erewrite IHHA; eauto.
+  Qed.
+
+  Next Obligation with mautosolve.
+  Qed.
+
+  Next Obligation with mautosolve.
+    enough {{ G ⊢ ℕ : Type@0 }} by intuition.
+    mauto.
+  Qed.
+
+  Next Obligation with mautosolve.
+    mauto 4 using lift_exp_max_right.
+  Qed.
+
+  Next Obligation with mautosolve.
+    enough {{ G ⊢ Type@j ⊆ A }} by contradiction.
+    assert {{ G ⊢ Type@0 ⊆ A }} by (apply wf_nat_inversion; mauto).
+    assert (exists l k, 0 <= k /\ {{ G ⊢ A ≈ Type@k : Type@l }}) as [? [k []]] by eauto using typ_subsumption_left_typ.
+    assert (j <= k) by mauto.
+    assert {{ G ⊢ Type@j ⊆ Type@k }} by mauto 4.
+    mauto 4.
+  Qed.
+
+  Next Obligation with mautosolve.
+    enough {{ G ⊢ Type@j : Type@(S j) }} by intuition.
+    mauto 4.
+  Qed.
+
+  Next Obligation with mautosolve.
+    mauto 4 using lift_exp_max_right.
+  Qed.
+
+  Next Obligation with mautosolve.
+    enough {{ G ⊢ Type@k ⊆ A }} by contradiction.
+    assert {{ G ⊢ Type@(S j) ⊆ A }} by (apply wf_typ_inversion; mauto).
+    assert (k <= (S j)) by mauto.
+    assert {{ G ⊢ Type@k ⊆ Type@(S j) }} by mauto 4.
+    mauto 4.
+  Qed.
+
+  Next Obligation with mautosolve.
+    intuition.
+  Qed.
+
+  Next Obligation with mautosolve.
+  Qed.
+
+  Next Obligation with mautosolve.
+    enough (exists i, {{ G ⊢ B' : Type@i }}) as [] by firstorder.
+    assert (exists C', {{ G, B' ⊢ M' : C' }} /\ {{ G ⊢ Π B' C' ⊆ A }}) as [? []] by mauto using wf_fn_inversion...
+  Qed.
+
+  Next Obligation with mautosolve.
+    gen_presups.
+    assert {{ G ⊢ B : Type@i }} by (eapply wf_pi_inversion'; eauto).
+    impl_obl_tac.
+  Qed.
+
+  Next Obligation with mautosolve.
+    enough {{ G ⊢ B' ≈ B : Type @ (Nat.max i j) }} by firstorder.
+    assert (exists C', {{ G, B' ⊢ M' : C' }} /\ {{ G ⊢ Π B' C' ⊆ A }}) as [C' []] by mauto using wf_fn_inversion.
+    TODOtac "Pi equivalence is invertible".
+  Qed.
+
+  Next Obligation with mautosolve.
+    gen_presups.
+    assert {{ ⊢ G, B' ≈ G, B }} by mauto 3.
+    enough {{ G, B ⊢ C : Type@i }} by mauto 3.
+    eapply wf_pi_inversion'; eauto.
+  Qed.
+
+  Next Obligation with mautosolve.
+    assert (exists C', {{ G, B' ⊢ M' : C' }} /\ {{ G ⊢ Π B' C' ⊆ A }}) as [C' []] by mauto using wf_fn_inversion.
+    TODOtac "Pi equivalence is invertible".
+  Qed.
+
+  Next Obligation with mautosolve.
+    gen_presups.
+    assert {{ G ⊢ Π B C : Type@i }} by (gen_presups; eauto).
+    assert {{ G, B ⊢ C : Type@i }} by (eapply wf_pi_inversion'; mauto 3).
+    assert {{ ⊢ G, B' ≈ G, B }} by mauto 3.
+    assert {{ G, B' ⊢ C : Type@i }} by mauto 3.
+    enough {{ G ⊢ Π B' C ≈ Π B C : Type@(max i j) }} by mauto.
+    econstructor; mauto 3.
+    enough {{ G, B' ⊢ C : Type@(max i j) }} by mauto 3.
+    impl_obl_tac.
+  Qed.
+
+  Next Obligation with mautosolve.
+    assert (exists C', {{ G, B' ⊢ M' : C' }} /\ exists j, {{ G ⊢ Π B' C' ≈ A : Type@j }}) as [C' [? []]] by mauto using wf_fn_inversion'.
+    firstorder.
+  Qed.
+
+  Next Obligation with mautosolve.
+  Qed.
+
+  Next Obligation with mautosolve.
+    gen_presups.
+    eapply wf_pi_inversion'; eauto.
+  Qed.
+
+  Next Obligation with mautosolve.
+    enough {{ G ⊢ N' : B' }} by contradiction.
+    assert (exists B' A' : typ, {{ G ⊢ M' : Π B' A' }} /\ {{ G ⊢ N' : B' }} /\ {{ G ⊢ ~ (a_sub A' {{{ Id,, N' }}}) ⊆ A }}) as [B'' [A'']] by mauto.
+    destruct_conjs.
+    gen_presups.
+    eapply wf_pi_inversion'; eauto.
+  Qed.
+
+  Next Obligation with mautosolve.
+    assert {{ G ⊢s Id,,M' : G, ℕ }} by mauto.
+    mauto using lift_exp_max_right.
+  Qed.
+
+  Next Obligation with mautosolve.
+    mauto using lift_exp_max_left.
+  Qed.
+
+  Next Obligation with mautosolve.
+    enough {{ G ⊢ A'[Id,,M'] ⊆ A }} by contradiction.
+    eapply wf_natrec_inversion...
+  Qed.
+
+  Next Obligation with mautosolve.
+    enough {{ G ⊢ MZ : A'[Id,,zero] }} by contradiction.
+    eapply wf_natrec_inversion...
+  Qed.
+
+  Next Obligation with mautosolve.
+    enough {{ G, ℕ, A' ⊢ MS : A'[Wk∘Wk,,succ #1] }} by contradiction.
+    eapply wf_natrec_inversion...
+  Qed.
+
+  Next Obligation with mautosolve.
+    apply lift_exp_max_right...
+  Qed.
+
+  Next Obligation with mautosolve.
+    apply lift_exp_max_left...
+  Qed.
+
+  Next Obligation with mautosolve.
+    apply lift_exp_max_right...
+  Qed.
+
+  Next Obligation with mautosolve.
+    apply lift_exp_max_left...
+  Qed.
+
+  Next Obligation with mautosolve.
+    enough (exists i, {{ G ⊢ A' : Type@i }}) as [] by firstorder.
+    assert (exists i B', {{ G ⊢ A' : Type@i }} /\ {{ G, A' ⊢ B' : Type@i }} /\ {{ G, A' ⊢ M' : B' }} /\ {{ G ⊢ Π A' B' ≈ A : Type@i }}) by mauto using wf_fn_inversion.
+    destruct_conjs...
+  Qed.
+
+  Next Obligation with mautosolve.
+    enough (exists B', {{ G, A' ⊢ M' : B' }}) as [] by firstorder.
+    assert (exists i B', {{ G ⊢ A' : Type@i }} /\ {{ G, A' ⊢ B' : Type@i }} /\ {{ G, A' ⊢ M' : B' }} /\ {{ G ⊢ Π A' B' ≈ A : Type@i }}) by mauto using wf_fn_inversion.
+    destruct_conjs...
+  Qed.
+
+  Next Obligation with mautosolve.
+    rename e into B'.
+    apply lift_exp_max_right...
+  Qed.
+
+  Next Obligation with mautosolve.
+    apply lift_exp_max_left...
+  Qed.
+
+  Next Obligation with mautosolve.
+    (* This case is not true! The implementation for lambda should be fixed. *)
+    rename e into B'.
+    enough {{ G ⊢ Π A' B' ⊆ A }} by contradiction.
+    assert (exists i B', {{ G ⊢ A' : Type@i }} /\ {{ G, A' ⊢ B' : Type@i }} /\ {{ G, A' ⊢ M' : B' }} /\ {{ G ⊢ Π A' B' ≈ A : Type@i }}) by mauto using wf_fn_inversion.
+    destruct_conjs.
+  Abort.
+
+  (* Next Obligation. mauto. Qed. *)
+  (* Next Obligation. mauto. Qed. *)
+
+  (* Next Obligation with mautosolve. *)
+  (*   enough {{ G ⊢ B : Type@i }} by firstorder. *)
+  (*   eapply wf_pi_inversion'... *)
+  (* Qed. *)
+
+  (* Next Obligation with mautosolve. *)
+  (*   enough {{ G, B ⊢ C : Type@i0 }} by firstorder. *)
+  (*   eapply wf_pi_inversion'... *)
+  (* Qed. *)
+
+  (* Next Obligation. mauto. Qed. *)
+End type_check.
